\documentclass[12pt, a4paper]{article}

\usepackage{geometry}
\geometry{verbose,a4paper,tmargin=2cm,bmargin=2cm,lmargin=2.5cm,rmargin=1.5cm}
 
\usepackage[english]{babel}
\usepackage{amsmath}
\usepackage{mathtools}
\usepackage{cases}
\usepackage{hyperref}

\begin{document}

	\section{SIR Model with natural deaths and births}

	Let's rewrite our system of equations \eqref{eq:dsdt} -- \eqref{eq:drdt} with an addition of the death and birth processes. Consider these rates are equal to each other, we introduce new variable $D$:
	\begin{numcases}{}
		\frac{ds(t)}{dt} = - \frac{\beta}{N} s(t) i(t) + D(N - s(t)) \label{eq:death_s} \\
		\frac{di(t)}{dt} = (\frac{\beta}{N} s(t) - \gamma - D) i(t) \label{eq:death_i} \\
		\frac{dr(t)}{dt} = \gamma i(t) - Dr(t) \label{eq:death_r}
	\end{numcases}
	As we did before, we rewrite it into one equation:
	\begin{equation} \label{eq:re_death_s}
		i = \frac{s' - D(N- s)}{-\tilde{\beta}s}
	\end{equation}
	Again we differentiate both sides (with $\tilde{\beta} = \frac{\beta}{N}$ substitution):
	\begin{equation}
		i' = -\frac{1}{\tilde{\beta}}(\frac{(s'' + D s')s - (s' + D s - D N)s'}{s^2}),
	\end{equation}
	\begin{equation} \label{eq:re_death_s_diff}	
		i' = -\frac{1}{\tilde{\beta}}(\frac{s''}{s} - \frac{s'^2 - D N s'}{s^2})
	\end{equation} 
	Now we can insert \eqref{eq:re_death_s} into \eqref{eq:death_i}:
	\begin{equation}
		i' = (\tilde{\beta} s - \gamma - D)(\frac{s' - D(N- s)}{-\tilde{\beta}s})
	\end{equation}
	\begin{equation} \label{eq:re_death_i_sub}
		i' = -\frac{1}{\tilde{\beta}s}(\tilde{\beta}s - \gamma - D)(s' + D s - D N)
	\end{equation}
	And comparing \eqref{eq:re_death_i_sub} and \eqref{eq:re_death_s_diff} we get next equation:
	\begin{equation} 
		s s'' - s'^2 +(-\tilde{\beta}s^2 + (\gamma + D)s + D N)s' - \tilde{\beta}D s^3 - (\tilde{\beta}D N + D(\gamma + D))s^2 - (\gamma + D)D N s = 0
	\end{equation}
	We can see that coefficients at $s^3, s^2$ and $s$ are $consts$ so we substitute them with \\ 
	$A = -\tilde{\beta}D, B = - (\tilde{\beta}D N + D(\gamma + D)),  C = - (\gamma + D)D N$:
	\begin{equation} \label{eq:death_main}
		s s'' - s'^2 +(-\tilde{\beta}s^2 + (\gamma + D)s + D N)s' +A s^3 + B s^2 + C s = 0
	\end{equation}
	Now we introduce a function $\phi = \frac{dt}{ds}$, so the equation will be:
	\begin{equation} \label{eq:death_main_phi}
		-\phi' - \frac{\phi}{s} +(-\tilde{\beta}s^2 + (\gamma + D)s + D N)\frac{\phi^2}{s} + (A s^2 + B s + C)\phi^3 = 0
	\end{equation}
	And by substitution $v = \phi s, v' = \phi's + \phi$ the following equation occur:
	\begin{equation} \label{eq:death_main_v}
		v' +(-\tilde{\beta} + \frac{(\gamma + D)}{s} + \frac{D N}{s^2})v^2 + (A + \frac{B}{s} + \frac{C}{s^2})v^3 = 0
	\end{equation}

	\newpage
	Then we assume these three substitutions:
	\begin{numcases}{}
		r(s) = \frac{1}{v(s)}, \\
		\xi(s) = (\tilde{\beta} - \frac{(\gamma + D)}{s} - \frac{D N}{s^2}), \\
		\eta(s) = -(A + \frac{B}{s} + \frac{C}{s^2})
	\end{numcases}
	and we get Abel-type first-order second-kind equation:
	\begin{equation}
		r r' = \xi(s)r + \eta(s)
	\end{equation}

\end{document}